WellFormed2.v
@@ -17,6 +17,783 @@ Require Import WellFormed.
 Module NatMapFacts := NatMapProperties.F.
 Module CacheletMapFacts := CacheletMapProperties.F.
 
+Definition wf3 (sigma: runtime_state): Prop :=
+  forall k mu rho pi lambda F V C R c e ranV,
+  (sigma = runtime_state_value k mu rho pi) ->
+  (NatMap.find lambda k = Some (single_level_cache F V C R)) ->
+  (V_range V e = Some ranV) ->
+  ((In c ranV -> ~In c F) /\ (In c F -> ~In c ranV)).
+
+(* WF3 MLC Read *)
+Lemma wf3_mlc_read : forall lambda h_tree k e' m0 l0 D obs1 mu k' index psi psi'
+  F V C R F' V' C' R' c enc ranV ranV',
+  well_defined_cache_tree h_tree ->
+  mlc_read k e' m0 l0 lambda h_tree = mlc_read_valid D obs1 mu k' ->
+  NatMap.find index k = Some psi ->
+  NatMap.find index k' = Some psi' ->
+  psi = single_level_cache F V C R ->
+  psi' = single_level_cache F' V' C' R' ->
+  V_range V enc = Some ranV ->
+  V_range V' enc = Some ranV' ->
+  ((In c ranV -> ~In c F) /\ (In c F -> ~In c ranV)) ->
+  ((In c ranV' -> ~In c F') /\ (In c F' -> ~In c ranV')).
+Proof.
+  unfold mlc_read.
+  intros lambda h_tree.
+  case_eq (get_cache_ID_path lambda h_tree).
+  intros l.
+  generalize dependent lambda.
+  induction l.
+  {
+    intros.
+    unfold recursive_mlc_read in H1.
+    subst.
+    destruct l0.
+    destruct (NatMap.find b m0).
+    injection H1; intros; subst.
+    rewrite -> H2 in H3.
+    injection H3; intros; subst.
+    rewrite -> H6 in H7.
+    injection H7; intros; subst.
+    exact H8.
+    discriminate.
+  }
+  {
+    intros lambda IHTREE. intros.
+    unfold recursive_mlc_read in H0.
+    fold recursive_mlc_read in H0.
+    case_eq (NatMap.find a k). intros.
+    assert (A0 := H8). destruct (NatMap.find a k) in A0, H0.
+    case_eq (cc_hit_read s0 e' l0). intros.
+    assert (A1 := H9). destruct (cc_hit_read s0 e' l0) in A1, H0.
+    injection H0; injection A0; injection A1; intros; subst; clear A0 A1.
+    assert (H10 := H9).
+    destruct s; destruct s1.
+    apply (cc_hit_read_f (single_level_cache c1 v w s) e' l0 D obs1 c0
+    (single_level_cache c2 v0 w0 s0) c1 v w s c2 v0 w0 s0) in H9.
+    apply (cc_hit_read_v (single_level_cache c1 v w s) e' l0 D obs1 c0
+    (single_level_cache c2 v0 w0 s0) c1 v w s c2 v0 w0 s0) in H10.
+    subst.
+    {
+      case_eq (eqb a index).
+      {
+        intros. apply cmp_to_eq in H3. subst.
+        rewrite -> H1 in H8.
+        injection H8; intros; subst c2 v0 w s.
+        assert (NatMap.find index (NatMap.add index (single_level_cache F V w0 s0) k) =
+        Some (single_level_cache F V w0 s0)).
+        apply NatMapFacts.add_eq_o. reflexivity.
+        rewrite -> H3 in H2.
+        injection H2; intros; subst F' V' w0 s0.
+        rewrite -> H5 in H6; injection H6; intros; subst.
+        exact H7.
+      }
+      {
+        intros. apply cmp_to_uneq in H3.
+        assert (NatMap.find index (NatMap.add a (single_level_cache c2 v0 w0 s0) k) = NatMap.find index k).
+        apply NatMapFacts.add_neq_o. exact H3.
+        rewrite -> H2 in H4.
+        rewrite -> H1 in H4.
+        injection H4; intros; subst F' V' C' R'.
+        rewrite -> H5 in H6; injection H6; intros; subst.
+        exact H7.
+      }
+    }
+    reflexivity.
+    reflexivity.
+    reflexivity.
+    reflexivity.
+    discriminate.
+    intros; destruct (cc_hit_read s0 e' l0).
+    discriminate.
+    case_eq (recursive_mlc_read k e' m0 l0 l). intros.
+    assert (A1 := H10). destruct (recursive_mlc_read k e' m0 l0 l) in A1, H0.
+    case_eq (cc_update s0 e' d1 l0). intros.
+    assert (A2 := H11). destruct (cc_update s0 e' d1 l0) in A2, H0.
+    injection H0; injection A0; injection A1; injection A2; intros; subst; clear A0 A1 A2.
+    {
+      case_eq (eqb index a).
+      {
+        intros. apply cmp_to_eq in H3. subst a.
+        destruct s.
+        assert (H12 := H11).
+        destruct s1.
+        apply (cc_update_f (single_level_cache c1 v w s) e' D l0 c0 (single_level_cache c2 v0 w0 s0)
+        c1 v w s c2 v0 w0 s0) in H11.
+        apply (cc_update_v (single_level_cache c1 v w s) e' D l0 c0 (single_level_cache c2 v0 w0 s0)
+        c1 v w s c2 v0 w0 s0) in H12.
+        subst.
+        assert (NatMap.find index (NatMap.add index (single_level_cache c2 v0 w0 s0) m) =
+        Some (single_level_cache c2 v0 w0 s0)).
+        apply NatMapFacts.add_eq_o. reflexivity.
+        rewrite -> H3 in H2.
+        rewrite -> H8 in H1.
+        injection H1; injection H2; intros; subst.
+        rewrite -> H5 in H6; injection H6; intros; subst.
+        exact H7.
+        reflexivity.
+        reflexivity.
+        reflexivity.
+        reflexivity.
+      }
+      {
+        intros. apply cmp_to_uneq in H3.
+        assert (WFH := H).
+        unfold well_defined_cache_tree in H.
+        destruct H as [ WFH1 ]. destruct H as [ WFH2 ]. destruct H as [ WFH3 ].
+        destruct l.
+        {
+          apply (IHl root_node WFH1 k e' m0 l0 D obs1 o m index (single_level_cache F V C R)
+          (single_level_cache F' V' C' R') F V C R F' V' C' R' c enc ranV ranV').
+          exact WFH.
+          unfold mlc_write. exact H10.
+          exact H1.
+          rewrite <- H2. apply eq_sym.
+          apply NatMapFacts.add_neq_o.
+          apply not_eq_sym. exact H3.
+          reflexivity.
+          reflexivity.
+          exact H5.
+          exact H6.
+          exact H7.
+        }
+        {
+          destruct lambda.
+          rewrite -> WFH1 in IHTREE. discriminate.
+          specialize (WFH3 c1 a (p :: l) IHTREE).
+          unfold get_cache_ID_path in IHTREE. discriminate.
+          specialize (WFH2 p0 a (p :: l) IHTREE).
+          injection WFH2; intros; subst.
+          apply (H p0 p l) in IHTREE.
+          apply (IHl (cache_node p) IHTREE k e' m0 l0 D obs1 o m index (single_level_cache F V C R)
+          (single_level_cache F' V' C' R') F V C R F' V' C' R' c enc ranV ranV').
+          exact WFH.
+          unfold mlc_write. exact H10.
+          exact H1.
+          rewrite <- H2. apply eq_sym.
+          apply NatMapFacts.add_neq_o.
+          apply not_eq_sym. exact H3.
+          reflexivity.
+          reflexivity.
+          exact H5.
+          exact H6.
+          exact H7.
+        }
+      }
+    }
+    discriminate.
+    intros; destruct (cc_update s0 e' d1 l0).
+    discriminate.
+    discriminate.
+    discriminate.
+    intros; destruct (recursive_mlc_read k e' m0 l0 l).
+    discriminate.
+    discriminate.
+    discriminate.
+    intros; destruct (NatMap.find a k).
+    discriminate.
+    discriminate.
+  }
+  intros; destruct (get_cache_ID_path lambda h_tree).
+  discriminate.
+  discriminate.
+Qed.
+
+(* WF3 MLC Allocation *)
+
+(* WF3 MLC Write *)
+Lemma wf3_mlc_write : forall lambda h_tree k e' m0 l0 v D obs1 mu k' index psi psi'
+  F V C R F' V' C' R' c enc ranV ranV',
+  well_defined_cache_tree h_tree ->
+  mlc_write k e' m0 l0 v lambda h_tree = mlc_write_valid D obs1 mu k' ->
+  NatMap.find index k = Some psi ->
+  NatMap.find index k' = Some psi' ->
+  psi = single_level_cache F V C R ->
+  psi' = single_level_cache F' V' C' R' ->
+  V_range V enc = Some ranV ->
+  V_range V' enc = Some ranV' ->
+  ((In c ranV -> ~In c F) /\ (In c F -> ~In c ranV)) ->
+  ((In c ranV' -> ~In c F') /\ (In c F' -> ~In c ranV')).
+Proof.
+  unfold mlc_write.
+  intros lambda h_tree.
+  case_eq (get_cache_ID_path lambda h_tree).
+  intros l.
+  generalize dependent lambda.
+  induction l.
+  {
+    intros lambda IHTREE k e' m0 l0 v D obs1 mu k' index psi psi'
+    F V C R F' V' C' R' c enc ranV ranV' WFH1; intros.
+    destruct (get_cache_ID_path lambda h_tree).
+    injection IHTREE; intros; subst.
+    unfold recursive_mlc_write in H.
+    subst. destruct l0.
+    destruct (NatMap.find b m0). destruct v.
+    discriminate.
+    injection H; intros; subst.
+    rewrite -> H0 in H1.
+    injection H1; intros; subst.
+    rewrite -> H4 in H5.
+    injection H5; intros; subst.
+    exact H6.
+    discriminate.
+    discriminate.
+  }
+  {
+    intros lambda IHTREE k e' m0 l0 v D obs1 mu k' index psi psi'
+    F V C R F' V' C' R' c enc ranV ranV' WFH1; intros.
+    unfold recursive_mlc_write in H.
+    fold recursive_mlc_write in H.
+    case_eq (NatMap.find a k). intros.
+    assert (A0 := H7). destruct (NatMap.find a k) in A0, H.
+    case_eq (cc_hit_write s0 e' l0 v). intros.
+    assert (A1 := H8). destruct (cc_hit_write s0 e' l0 v) in A1, H. destruct l0.
+    injection H; injection A0; injection A1; intros; subst; clear A0 A1.
+    assert (H9 := H8).
+    destruct s; destruct s1.
+    apply (cc_hit_write_f (single_level_cache c1 v0 w s) e' (address b d1) v D c0
+    (single_level_cache c2 v1 w0 s0) c1 v0 w s c2 v1 w0 s0) in H8.
+    apply (cc_hit_write_v (single_level_cache c1 v0 w s) e' (address b d1) v D c0
+    (single_level_cache c2 v1 w0 s0) c1 v0 w s c2 v1 w0 s0) in H9.
+    subst.
+    {
+      case_eq (eqb a index).
+      {
+        intros. apply cmp_to_eq in H2. subst.
+        rewrite -> H0 in H7.
+        injection H7; intros; subst c2 v1 w s.
+        assert (NatMap.find index (NatMap.add index (single_level_cache F V w0 s0) k) =
+        Some (single_level_cache F V w0 s0)).
+        apply NatMapFacts.add_eq_o. reflexivity.
+        rewrite -> H2 in H1.
+        injection H1; intros; subst F' V' w0 s0.
+        rewrite -> H4 in H5; injection H5; intros; subst.
+        exact H6.
+      }
+      {
+        intros. apply cmp_to_uneq in H2.
+        assert (NatMap.find index (NatMap.add a (single_level_cache c2 v1 w0 s0) k) = NatMap.find index k).
+        apply NatMapFacts.add_neq_o. exact H2.
+        rewrite -> H1 in H3.
+        rewrite -> H0 in H3.
+        injection H3; intros; subst F' V' C' R'.
+        rewrite -> H4 in H5; injection H5; intros; subst.
+        exact H6.
+      }
+    }
+    reflexivity.
+    reflexivity.
+    reflexivity.
+    reflexivity.
+    discriminate.
+    intros; destruct (cc_hit_write s0 e' l0).
+    discriminate.
+    case_eq (recursive_mlc_write k e' m0 l0 v l). intros.
+    assert (A1 := H9). destruct (recursive_mlc_write k e' m0 l0 v l) in A1, H.
+    case_eq (cc_update s0 e' d0 l0). intros.
+    assert (A2 := H10). destruct (cc_update s0 e' d0 l0) in A2, H.
+    injection H; injection A0; injection A1; injection A2; intros; subst; clear A0 A1 A2.
+    {
+      case_eq (eqb index a).
+      {
+        intros. apply cmp_to_eq in H2. subst a.
+        destruct s.
+        assert (H11 := H10).
+        destruct s1.
+        apply (cc_update_f (single_level_cache c1 v0 w s) e' D l0 c0 (single_level_cache c2 v1 w0 s0)
+        c1 v0 w s c2 v1 w0 s0) in H10.
+        apply (cc_update_v (single_level_cache c1 v0 w s) e' D l0 c0 (single_level_cache c2 v1 w0 s0)
+        c1 v0 w s c2 v1 w0 s0) in H11.
+        subst.
+        assert (NatMap.find index (NatMap.add index (single_level_cache c2 v1 w0 s0) m1) =
+        Some (single_level_cache c2 v1 w0 s0)).
+        apply NatMapFacts.add_eq_o. reflexivity.
+        rewrite -> H2 in H1.
+        rewrite -> H7 in H0.
+        injection H0; injection H1; intros; subst.
+        rewrite -> H4 in H5; injection H5; intros; subst.
+        exact H6.
+        reflexivity.
+        reflexivity.
+        reflexivity.
+        reflexivity.
+      }
+      {
+        intros. apply cmp_to_uneq in H2.
+        assert (WFH := WFH1).
+        unfold well_defined_cache_tree in WFH1.
+        destruct WFH1 as [ WFH1 WFH2 ]. destruct WFH2 as [ WFH2 WFH3 ]. destruct WFH3 as [ WFH3 WFH4 ].
+        destruct l.
+        {
+          apply (IHl root_node WFH1 k e' m0 l0 v D o mu m1 index (single_level_cache F V C R)
+          (single_level_cache F' V' C' R') F V C R F' V' C' R' c enc ranV ranV').
+          exact WFH.
+          unfold mlc_write. exact H9.
+          exact H0.
+          rewrite <- H1. apply eq_sym.
+          apply NatMapFacts.add_neq_o.
+          apply not_eq_sym. exact H2.
+          reflexivity.
+          reflexivity.
+          exact H4.
+          exact H5.
+          exact H6.
+        }
+        {
+          destruct lambda.
+          rewrite -> WFH1 in IHTREE. discriminate.
+          specialize (WFH3 c1 a (p :: l) IHTREE).
+          unfold get_cache_ID_path in IHTREE. discriminate.
+          specialize (WFH2 p0 a (p :: l) IHTREE).
+          injection WFH2; intros; subst.
+          apply (WFH4 p0 p l) in IHTREE.
+          apply (IHl (cache_node p) IHTREE k e' m0 l0 v D o mu m1 index (single_level_cache F V C R)
+          (single_level_cache F' V' C' R') F V C R F' V' C' R' c enc ranV ranV').
+          exact WFH.
+          unfold mlc_write. exact H9.
+          exact H0.
+          rewrite <- H1. apply eq_sym.
+          apply NatMapFacts.add_neq_o.
+          apply not_eq_sym. exact H2.
+          reflexivity.
+          reflexivity.
+          exact H4.
+          exact H5.
+          exact H6.
+        }
+      }
+    }
+    discriminate.
+    intros; destruct (cc_update s0 e' d0 l0).
+    discriminate.
+    discriminate.
+    discriminate.
+    intros; destruct (recursive_mlc_write k e' m0 l0 v l).
+    discriminate.
+    discriminate.
+    discriminate.
+    intros; destruct (NatMap.find a k).
+    discriminate.
+    discriminate.
+  }
+  intros; destruct (get_cache_ID_path lambda h_tree).
+  discriminate.
+  discriminate.
+Qed.
+
+(* WF3 MLC Deallocation *)
+Lemma clear_remapping_list_v : forall r r1 F V C R F' V' C' R' enc,
+  NatMap.In r V ->
+  clear_remapping_list r (NatMapProperties.to_list r1) F V C R = Some (single_level_cache F' V' C' R') ->
+  (NatMap.In enc V <-> NatMap.In enc V').
+Proof.
+  intros r r0.
+  induction (NatMapProperties.to_list r0).
+  {
+    intros.
+    unfold clear_remapping_list in H0.
+    injection H0; intros; subst.
+    split.
+    intros.
+    apply NatMapFacts.add_in_iff.
+    right. exact H1.
+    intros.
+    apply NatMapFacts.add_in_iff in H1.
+    destruct H1.
+    subst. exact H.
+    exact H1.
+  }
+  {
+    intros.
+    unfold clear_remapping_list in H0.
+    fold clear_remapping_list in H0.
+    case_eq a. intros.
+    destruct a.
+    injection H1; intros; subst k0 w0; clear H1.
+    case_eq (free_cachelets r k w F V C R); intros.
+    assert (A0 := H1). destruct (free_cachelets r k w F V C R) in A0, H0.
+    injection A0; intros; subst s0; clear A0.
+    destruct s.
+    apply (free_cachelets_v w r k F V C R c v w0 s) in H1. subst v.
+    apply (IHl c V w0 s F' V' C' R' enc).
+    exact H. exact H0.
+    discriminate.
+    destruct (free_cachelets r k w F V C R).
+    discriminate.
+    discriminate.
+  }
+Qed.
+
+Lemma V_range_add_empty : forall V r enc ranV ranV' c,
+  V_range V enc = Some ranV ->
+  V_range (NatMap.add r (NatMap.empty way_mask) V) enc = Some ranV' ->
+  In c ranV' -> In c ranV.
+Proof.
+  intros.
+  unfold V_range in *.
+  case_eq (NatMap.find enc V). intros.
+  assert (A0 := H2). destruct (NatMap.find enc V) in H, A0.
+  case_eq (NatMap.find (elt:=remapping_list) enc (NatMap.add r (NatMap.empty way_mask) V)). intros.
+  assert (A1 := H3). destruct (NatMap.find (elt:=remapping_list) enc (NatMap.add r (NatMap.empty way_mask) V)) in H0, A1.
+  injection A0; injection A1; intros; subst r3 r0; clear A0 A1.
+  case_eq (eqb r enc); intros.
+  apply cmp_to_eq in H4; subst r.
+  assert (NatMap.find (elt:=remapping_list) enc (NatMap.add enc (NatMap.empty way_mask) V) = Some (NatMap.empty way_mask)).
+  apply NatMapFacts.add_eq_o. reflexivity.
+  rewrite -> H3 in H4.
+  injection H4; intros; subst.
+  injection H0; intros; subst.
+  unfold In in H1. destruct H1.
+  apply cmp_to_uneq in H4.
+  assert (NatMap.find (elt:=remapping_list) enc (NatMap.add r (NatMap.empty way_mask) V)
+  = NatMap.find (elt:=remapping_list) enc V).
+  apply NatMapFacts.add_neq_o. exact H4.
+  rewrite -> H2 in H5.
+  rewrite -> H3 in H5.
+  injection H5; intros; subst r2.
+  rewrite -> H0 in H.
+  injection H; intros; subst ranV'.
+  exact H1.
+  discriminate.
+  intros; destruct (NatMap.find (elt:=remapping_list) enc (NatMap.add r (NatMap.empty way_mask) V)).
+  discriminate.
+  discriminate.
+  discriminate.
+  intros; destruct (NatMap.find enc V).
+  discriminate.
+  discriminate.
+Qed.
+
+Lemma wf3_free_cachelets : forall w0 r k F V C R F' V' C' R' r0 c enc ranV ranV',
+  ((In c ranV -> ~In c F) /\ (In c F -> ~In c ranV)) ->
+  V_range V enc = Some ranV ->
+  V_range V' enc = Some ranV' ->
+  NatMap.find r V = Some r0 ->
+  free_cachelets r k w0 F V C R = Some (single_level_cache F' V' C' R') ->
+  ((In c ranV' -> ~In c F') /\ (In c F' -> ~In c ranV')).
+Proof.
+  intros w0.
+  induction w0.
+  {
+    intros.
+    unfold free_cachelets in H3.
+    injection H3; intros; subst.
+    rewrite -> H0 in H1.
+    injection H1; intros; subst.
+    exact H.
+  }
+  {
+    intros.
+    unfold free_cachelets in H3.
+    fold free_cachelets in H3.
+    case_eq (NatMap.find k R). intros.
+    assert (A0 := H4). destruct (NatMap.find k R) in A0, H3.
+    case_eq (cachelet_invalidation C (a, k)). intros.
+    assert (A1 := H5). destruct (cachelet_invalidation C (a, k)) in A1, H3.
+    injection A0; injection A1; intros; subst p0 w1; clear A0 A1.
+    apply (IHw0 r k ((a, k) :: F) V w (NatMap.add k (update p a (enclave_ID_active r)) R)
+    F' V' C' R' r0 c enc ranV ranV').
+    destruct H.
+    split.
+    {
+      intros.
+      intros contra.
+      apply in_inv in contra.
+      destruct contra.
+      give_up.
+      apply H6 in H8.
+      apply H8 in H7.
+      exact H7.
+    }
+    give_up.
+    give_up.
+    give_up.
+    give_up.
+    give_up.
+    give_up.
+    give_up.
+    give_up.
+    give_up.
+  }
+Admitted.
+
+Lemma wf3_clear_remapping_list : forall r r1 F V C R F' V' C' R' c enc ranV ranV',
+  ((In c ranV -> ~In c F) /\ (In c F -> ~In c ranV)) ->
+  V_range V enc = Some ranV ->
+  V_range V' enc = Some ranV' ->
+  NatMap.In r V ->
+  clear_remapping_list r (NatMapProperties.to_list r1) F V C R = Some (single_level_cache F' V' C' R') ->
+  ((In c ranV' -> ~In c F') /\ (In c F' -> ~In c ranV')).
+Proof.
+  intros r r0.
+  induction (NatMapProperties.to_list r0).
+  {
+    intros.
+    assert (H4 := H3).
+    apply (clear_remapping_list_v r (NatMap.empty way_mask) F V C R F' V' C' R' enc) in H4.
+    unfold clear_remapping_list in H3.
+    injection H3; intros; subst F' V' C' R'.
+    assert (In c ranV' -> In c ranV).
+    apply (V_range_add_empty V r enc ranV ranV' c).
+    exact H0. exact H1.
+    destruct H.
+    split.
+    {
+      intros.
+      apply H.
+      apply H5.
+      exact H7.
+    }
+    {
+      intros.
+      intros contra.
+      apply H5 in contra.
+      apply H in contra.
+      apply contra in H7.
+      destruct H7.
+    }
+    exact H2.
+  }
+  {
+    intros.
+    unfold clear_remapping_list in H3.
+    fold clear_remapping_list in H3.
+    destruct a.
+    case_eq (free_cachelets r k w F V C R). intros.
+    assert (A0 := H4). destruct (free_cachelets r k w F V C R) in A0, H3.
+    destruct s; destruct s0.
+    injection A0; intros; subst; clear A0.
+    give_up.
+    give_up.
+    give_up.
+  }
+Admitted.
+
+
+Lemma wf3_mlc_dealloc : forall lambda h_tree state k k' index psi psi' F V C R F' V' C' R' c enc ranV ranV',
+  well_defined_cache_tree h_tree ->
+  mlc_deallocation state k lambda h_tree = Some k' ->
+  NatMap.find index k = Some psi ->
+  NatMap.find index k' = Some psi' ->
+  psi = single_level_cache F V C R ->
+  psi' = single_level_cache F' V' C' R' ->
+  V_range V enc = Some ranV ->
+  V_range V' enc = Some ranV' ->
+  ((In c ranV -> ~In c F) /\ (In c F -> ~In c ranV)) ->
+  ((In c ranV' -> ~In c F') /\ (In c F' -> ~In c ranV')).
+Proof.
+  unfold mlc_deallocation.
+  intros lambda h_tree state.
+  case_eq (get_cache_ID_path lambda h_tree).
+  intros l.
+  generalize dependent lambda.
+  induction l.
+  {
+    intros lambda IHTREE k k' index psi psi' F V C R
+    F' V' C' R' c enc ranV ranV' WFH; intros.
+    destruct state; destruct e.
+    unfold recursive_mlc_deallocation in H.
+    injection H; intros; subst k'.
+    rewrite -> H0 in H1.
+    injection H1; intros; subst psi psi'.
+    injection H7; intros; subst F' V' C' R'.
+    rewrite -> H5 in H4; injection H4; intros; subst.
+    exact H6.
+    discriminate.
+  }
+  {
+    intros lambda IHTREE k k' index psi psi' F V C R
+    F' V' C' R' c enc ranV ranV' WFH; intros.
+    destruct state; destruct e.
+    unfold recursive_mlc_deallocation in H.
+    fold recursive_mlc_deallocation in H.
+    case_eq (NatMap.find a k). intros.
+    assert (A0 := H7). destruct (NatMap.find a k) in A0, H.
+    case_eq (cachelet_deallocation r s0). intros.
+    assert (A1 := H8). destruct (cachelet_deallocation r s0) in A1, H.
+    injection A0; injection A1; intros; subst s0 s2; clear A0 A1.
+    assert (WFH1 := WFH).
+    unfold well_defined_cache_tree in WFH1.
+    destruct WFH1 as [ WFH1 WFH2 ]. destruct WFH2 as [ WFH2 WFH3 ]. destruct WFH3 as [ WFH3 WFH4 ].
+    case_eq (eqb index a).
+    {
+      intros; apply cmp_to_eq in H9; subst a.
+      rewrite -> H7 in H0.
+      injection H0; intros; subst s.
+      destruct s1.
+      case_eq (V_range v enc). intros.
+      destruct l.
+      {
+        apply (IHl root_node WFH1 (NatMap.add index (single_level_cache c0 v w s) k) k' index
+        (single_level_cache c0 v w s) psi' c0 v w s F' V' C' R' c enc l0 ranV').
+        exact WFH.
+        unfold mlc_deallocation. exact H.
+        apply NatMapFacts.add_eq_o. reflexivity.
+        exact H1.
+        reflexivity.
+        exact H3.
+        exact H9.
+        exact H5.
+        unfold cachelet_deallocation in H8. destruct psi.
+        case_eq (NatMap.find r v0). intros.
+        assert (A0 := H10). destruct (NatMap.find r v0) in A0, H8.
+        injection A0; injection H2; intros; subst c1 v0 w0 s0 r1; clear A0.
+        (* apply (wf3_clear_remapping_list r r1 (single_level_cache c1 v0 w0 s0) (single_level_cache c0 v w s)
+        c1 v0 w0 s0 c0 v w s c) in H8. *)
+        give_up.
+        discriminate.
+        intros; destruct (NatMap.find r v0).
+        discriminate.
+        discriminate.
+      }
+      {
+        destruct lambda.
+        rewrite -> WFH1 in IHTREE. discriminate.
+        specialize (WFH3 c1 index (p :: l) IHTREE).
+        unfold get_cache_ID_path in IHTREE. discriminate.
+        specialize (WFH2 p0 index (p :: l) IHTREE).
+        injection WFH2; intros; subst p0.
+        apply (WFH4 index p l) in IHTREE.
+        apply (IHl (cache_node p) IHTREE (NatMap.add index (single_level_cache c0 v w s) k) k' index
+        (single_level_cache c0 v w s) psi' c0 v w s F' V' C' R' c enc l0 ranV').
+        exact WFH.
+        unfold mlc_deallocation. exact H.
+        apply NatMapFacts.add_eq_o. reflexivity.
+        exact H1.
+        reflexivity.
+        exact H3.
+        exact H9.
+        exact H5.
+        destruct psi.
+        (*
+        apply (wf2_cachelet_deallocation r psi (single_level_cache c0 v w s) F V C R
+        c0 v w s enc ranV l0 c).
+        exact H9. exact H2. reflexivity. exact H4.
+        exact H10. exact H6. exact H7.
+        *)
+        give_up.
+      }
+      {
+        intros. destruct psi.
+        injection H2; intros; subst c1 v0 w0 s0.
+        apply (cachelet_deallocation_v r (single_level_cache F V C R) (single_level_cache c0 v w s)
+        F V C R c0 v w s enc) in H8.
+        apply V_range_in in H4. apply V_range_not_in in H9.
+        apply H8 in H4.
+        apply H9 in H4.
+        destruct H4.
+        reflexivity.
+        reflexivity.
+      }
+    }
+    {
+      intros; apply cmp_to_uneq in H9.
+      destruct l.
+      {
+        apply (IHl root_node WFH1 (NatMap.add a s1 k) k' index
+        psi psi' F V C R F' V' C' R' c enc ranV ranV').
+        exact WFH.
+        unfold mlc_deallocation. exact H.
+        rewrite <- H0. apply NatMapFacts.add_neq_o.
+        apply not_eq_sym. exact H9.
+        exact H1.
+        exact H2.
+        exact H3.
+        exact H4.
+        exact H5.
+        exact H6.
+      }
+      {
+        destruct lambda.
+        rewrite -> WFH1 in IHTREE. discriminate.
+        specialize (WFH3 c0 a (p :: l) IHTREE).
+        unfold get_cache_ID_path in IHTREE. discriminate.
+        specialize (WFH2 p0 a (p :: l) IHTREE).
+        injection WFH2; intros; subst p0.
+        apply (WFH4 a p l) in IHTREE.
+        apply (IHl (cache_node p) IHTREE (NatMap.add a s1 k) k' index
+        psi psi' F V C R F' V' C' R' c enc ranV ranV').
+        exact WFH.
+        unfold mlc_deallocation. exact H.
+        rewrite <- H0. apply NatMapFacts.add_neq_o.
+        apply not_eq_sym. exact H9.
+        exact H1.
+        exact H2.
+        exact H3.
+        exact H4.
+        exact H5.
+        exact H6.
+      }
+    }
+    discriminate.
+    intros; destruct (cachelet_deallocation r s0).
+    discriminate.
+    discriminate.
+    discriminate.
+    intros; destruct (NatMap.find a k).
+    discriminate.
+    discriminate.
+    discriminate.
+  }
+  intros; destruct (get_cache_ID_path lambda h_tree).
+  discriminate.
+  destruct state; destruct e; discriminate.
+Admitted.
+
+Lemma wf3_preservation : forall sigma obs sigma' obs',
+  wf3 sigma -> <<sigma; obs>> ===> <<sigma'; obs'>> -> wf3 sigma'.
+Proof.
+  destruct sigma; destruct sigma'.
+  unfold wf3 in *.
+  intros; injection H1; intros.
+  inversion H0. inversion H19; subst.
+  - case_eq (NatMap.find lambda m); intros; subst.
+    destruct s.
+    case_eq (V_range v e); intros.
+    assert (V_range v e = Some l1 -> (In c l1 -> ~ In c c0) /\ (In c c0 -> ~In c l1)).
+    apply (H m mu rho p lambda c0 v w s c e l1). reflexivity. exact H4.
+    apply (wf3_mlc_read lambda0 h_tree m e' mu l0 D delta obs0 k lambda (single_level_cache c0 v w s)
+    (single_level_cache F V C R) c0 v w s F V C R c e l1 ranV).
+    exact H25. exact H36. exact H4. exact H2. reflexivity.
+    reflexivity. exact H5. exact H3. apply H6 in H5. exact H5.
+    apply (wf2_mlc_read_none lambda0 h_tree m e' mu l0 D delta obs0 k lambda (single_level_cache c0 v w s)
+    (single_level_cache F V C R) c0 v w s F V C R e) in H5.
+    rewrite -> H3 in H5. discriminate.
+    exact H25. exact H36. exact H4. exact H2. reflexivity.
+    reflexivity.
+    apply (wf_mlc_read_none lambda0 h_tree m e' mu l0 D delta obs0 k lambda) in H4.
+    rewrite -> H2 in H4.
+    discriminate. exact H25. exact H36.
+  - give_up.
+  - case_eq (NatMap.find lambda m); intros; subst.
+    destruct s.
+    case_eq (V_range v0 e); intros.
+    assert (V_range v0 e = Some l1 -> (In c l1 -> ~ In c c0) /\ (In c c0 -> ~In c l1)).
+    apply (H m m0 rho p lambda c0 v0 w s c e l1). reflexivity. exact H4.
+    apply (wf3_mlc_write lambda0 h_tree m e' m0 l0 v D obs1 mu k lambda (single_level_cache c0 v0 w s)
+    (single_level_cache F V C R) c0 v0 w s F V C R c e l1 ranV).
+    exact H25. exact H36. exact H4. exact H2. reflexivity.
+    reflexivity. exact H5. exact H3. apply H6 in H5. exact H5.
+    apply (wf2_mlc_write_none lambda0 h_tree m e' m0 l0 v D obs1 mu k lambda (single_level_cache c0 v0 w s)
+    (single_level_cache F V C R) c0 v0 w s F V C R) in H5.
+    rewrite -> H5 in H3. discriminate.
+    exact H25. exact H36. exact H4. exact H2. reflexivity. reflexivity.
+    apply (wf_mlc_write_none lambda0 h_tree m e' m0 l0 v D obs1 mu k lambda) in H4.
+    rewrite -> H4 in H2.
+    discriminate. exact H25. exact H36.
+  - give_up.
+  - apply (H k mu rho p lambda F V C R c e ranV).
+    reflexivity. exact H2. exact H3.
+  - apply (H k mu rho p lambda F V C R c e ranV).
+    reflexivity. exact H2. exact H3.
+  - apply (H k mu rho p lambda F V C R c e ranV).
+    reflexivity. exact H2. exact H3.
+  - apply (H k mu rho p lambda F V C R c e ranV).
+    reflexivity. exact H2. exact H3.
+  - subst. apply (H k mu rho p lambda F V C R c e ranV).
+    reflexivity. exact H2. exact H3.
+Admitted.
+
 Definition wf4 (sigma: runtime_state): Prop :=
   forall k mu rho pi p l q e E,
   (sigma = runtime_state_value k mu rho pi) ->
@@ -91,32 +868,58 @@ Proof.
 Qed.
 
 Lemma wf4_enclave_elimination : forall e E e' E' r,
-  ((enclave_elimination (enclave_state_value e E) r) = enclave_state_value e' E') ->
-  (exists raw_e, e = enclave_ID_active raw_e /\ NatMap.In raw_e E) ->
-  (exists raw_e', e' = enclave_ID_active raw_e' /\ NatMap.In raw_e' E').
+  ((enclave_elimination (enclave_state_value e E) r) = enclave_state_valid (enclave_state_value e' E')) ->
+  (e = enclave_ID_inactive \/ (exists raw_e, e = enclave_ID_active raw_e /\ NatMap.In raw_e E)) ->
+  (e = enclave_ID_inactive \/ (exists raw_e', e' = enclave_ID_active raw_e' /\ NatMap.In raw_e' E')).
 Proof.
   intros.
+  destruct H0. left. exact H0.
   destruct e'.
+  {
+    right.
+    unfold enclave_elimination in H.
+    destruct e.
+    case_eq (r =? r1); intros.
+    assert (A0 := H1). destruct (r =? r1) in H, A0.
+    discriminate.
+    discriminate.
+    intros. assert (H2 := H1). apply cmp_to_uneq in H1.
+    destruct (r =? r1).
+    discriminate.
+    injection H; intros; subst.
+    destruct H0.
+    destruct H0.
+    injection H0; intros; subst.
+    eexists x.
+    split. reflexivity.
+    apply NatMapFacts.remove_in_iff.
+    split. exact H1. exact H3.
+    destruct H0.
+    destruct H0.
+    discriminate.
+  }
+  {
+    unfold enclave_elimination in H.
+    destruct e.
+    destruct (r =? r0).
+    discriminate.
+    discriminate.
+    left. reflexivity.
+  }
+Qed.
+
+Lemma enclave_elimination_state : forall e E e' E' r,
+  ((enclave_elimination (enclave_state_value e E) r) = enclave_state_valid (enclave_state_value e' E')) ->
+  e = e'.
+Proof.
+  intros.
   unfold enclave_elimination in H.
-  injection H; intros; subst.
-  destruct H0.
-  destruct H0.
-  case_eq (eqb r x).
-  intros; apply cmp_to_eq in H2; subst.
-  eexists x. split. injection H0; intros; subst; reflexivity.
-  (* this case is actually not possible *)
-  give_up.
-  intros; apply cmp_to_uneq in H2.
-  injection H0; intros; subst.
-  destruct H0.
-  eexists x. split. reflexivity.
-  apply NatMapFacts.remove_in_iff.
-  split. exact H2. exact H1.
-  injection H; intros; subst.
-  destruct H0.
-  destruct H0.
+  destruct e.
+  destruct (r =? r0).
   discriminate.
-Admitted.
+  injection H; intros; subst; reflexivity.
+  injection H; intros; subst; reflexivity.
+Qed.
 
 Lemma wf4_preservation : forall sigma obs sigma' obs',
   wf4 sigma -> <<sigma; obs>> ===> <<sigma'; obs'>> -> wf4 sigma'.
@@ -155,7 +958,7 @@ Proof.
     reflexivity.
     exact H19.
     apply (wf4_enclave_creation e0 e1 e E mu n r_val2_addr r_val3).
-    exact H39.
+    exact H40.
     exact H4.
     intros; apply cmp_to_uneq in H3.
     assert (NatMap.find p1 (NatMap.add p2 (process_value e' l' q0) p) = NatMap.find p1 p).
@@ -181,18 +984,22 @@ Proof.
     rewrite <- H4. exact H2.
   - subst. case_eq (eqb p1 p2).
     intros. apply cmp_to_eq in H3. subst.
-    assert (NatMap.find p2 (NatMap.add p2 (process_value (enclave_elimination (enclave_state_value
-    (enclave_ID_active e_raw) mem) r_val) l' q0) p) = Some (process_value (enclave_elimination
-    (enclave_state_value (enclave_ID_active e_raw) mem) r_val) l' q0)).
+    assert (NatMap.find p2 (NatMap.add p2 (process_value e' l' q0) p)
+    = Some (process_value e' l' q0)).
     apply NatMapFacts.add_eq_o; reflexivity.
     rewrite -> H2 in H3.
     injection H3; intros; subst.
-    right.
-    (* issue with enclave elimination definition *)
-    give_up.
+    assert (H40 := H39).
+    apply (enclave_elimination_state (enclave_ID_active e_raw) mem e E r_val) in H40. subst e.
+    assert (enclave_ID_active e_raw = enclave_ID_inactive \/ (exists raw_e : raw_enclave_ID,
+    enclave_ID_active e_raw = enclave_ID_active raw_e /\ NatMap.In raw_e mem)).
+    apply (H m m0 rho p p2 l0 q0 (enclave_ID_active e_raw) mem).
+    reflexivity.
+    exact H19.
+    apply (wf4_enclave_elimination (enclave_ID_active e_raw) mem (enclave_ID_active e_raw) E r_val).
+    exact H39. exact H4.
     intros; apply cmp_to_uneq in H3.
-    assert (NatMap.find p1 (NatMap.add p2 (process_value (enclave_elimination (enclave_state_value
-    (enclave_ID_active e_raw) mem) r_val) l' q0) p) = NatMap.find p1 p).
+    assert (NatMap.find p1 (NatMap.add p2 (process_value e' l' q0) p) = NatMap.find p1 p).
     apply NatMapFacts.add_neq_o; apply not_eq_sym; exact H3.
     apply (H m m0 rho p p1 l q e E).
     reflexivity.
@@ -289,7 +1096,7 @@ Proof.
     apply (H k mu rho p p1 l q e E).
     reflexivity.
     rewrite <- H4. exact H2.
-Admitted.
+Qed.
 
 Definition wf5 (sigma: runtime_state): Prop :=
   forall k mu rho pi index F V C R p l q e E,
